new/golang/theory/dynamic_typing.v
@@ -3,12 +3,14 @@ From Coq Require Import Program.Equality.
 From Ltac2 Require Import Ltac2.
 Set Default Proof Mode "Classic".
 From New.golang.defn Require Export dynamic_typing.
-From New.golang.theory Require Import typing.
+From New.golang.theory Require Import typing list mem.
+From New.golang.theory Require Import proofmode.
 
 Set Default Proof Using "Type".
 
 Section goose_lang.
-Context `{ffi_syntax}.
+Context `{sem: ffi_semantics} `{!ffi_interp ffi} `{!heapGS Σ}.
+Context `{!IntoVal V}.
 
 #[global] Instance to_val_w64_inj : Inj eq eq (λ (n: w64), #n).
 Proof.
@@ -22,7 +24,7 @@ Proof.
   intros s1 s2. inv 1. auto.
 Qed.
 
-#[global] Instance type_to_val_inj : Inj eq eq type_to_val.
+#[global] Instance type_to_val_inj : Inj eq eq type.type_to_val.
 Proof.
   intros t1 t2.
   generalize dependent t2.
@@ -48,5 +50,120 @@ Proof.
       apply Hfields in Ht; subst; auto.
       apply IHdecls in Hdecls; [ inv Hdecls; auto | auto ].
 Qed.
+
+#[global] Instance descriptor_into_val : IntoVal (go_string * go_type) :=
+  { to_val_def := fun '(d, t) => (#d, #t)%V; }.
+
+Global Instance wp_type_Match (t : go_type) (baseCase arrayCase structCase : val) :
+  PureWp True
+    (type.Match #t baseCase arrayCase structCase)
+    (match t with
+     | arrayT n t => (arrayCase #n #t)%V
+     | structT d => (structCase #d)%V
+     | _ => (baseCase #t)%V
+     end).
+Proof.
+  rewrite type.Match_unseal.
+  intros ?????. iIntros "Hwp".
+  rewrite [in #t]to_val_unseal.
+  destruct t; wp_call_lc "?"; try by iApply "Hwp".
+  - rewrite to_val_unseal /=.
+    by iApply "Hwp".
+  - iDestruct ("Hwp" with "[$]") as "Hwp".
+    iExactEq "Hwp".
+    repeat f_equal.
+    repeat rewrite !to_val_unseal /=.
+    induction decls as [|[d t] decls]; simpl; auto.
+    congruence.
+Qed.
+
+Lemma wp_type_size' (t: go_type) stk E :
+  {{{ True }}}
+    type.go_type_size_e #t @ stk; E
+  {{{ RET (#(W64 (Z.of_nat (go_type_size t)))); £1 }}}.
+Proof.
+  rewrite type.go_type_size_e_unseal.
+  rewrite go_type_size_unseal.
+
+  induction t using go_type_ind; iIntros (Φ) "_ HΦ"; wp_call_lc "Hlc";
+    try iApply ("HΦ" with "Hlc").
+
+  - wp_apply IHt. iIntros "_". wp_pures.
+    iSpecialize ("HΦ" with "Hlc"). iExactEq "HΦ".
+    repeat f_equal.
+    simpl; word.
+  - iSpecialize ("HΦ" with "Hlc").
+    iInduction decls as [| [d t] decls ] forall (Φ); wp_pures.
+    + auto.
+    + rewrite [in #(d :: t)%struct]to_val_unseal /=.
+      wp_pures.
+      wp_apply Hfields.
+      { naive_solver. }
+      iIntros "_". wp_pures.
+      wp_bind (match decls with | nil => _ | cons _ _ => _ end).
+      iApply ("IHdecls" with "[] [HΦ]").
+      { iPureIntro. naive_solver. }
+      wp_pures.
+      iExactEq "HΦ".
+      repeat f_equal. word.
+Qed.
+
+Global Instance wp_type_size (t: go_type) :
+  PureWp True
+         (type.go_type_size_e #t)
+         (#(W64 (Z.of_nat (go_type_size t)))).
+Proof.
+  intros ?????; iIntros "Hwp".
+  wp_apply wp_type_size'. iIntros "?".
+  iApply ("Hwp" with "[$]").
+Qed.
+
+Context `{!IntoValTyped V t}.
+
+Lemma wp_load_ty l (v: V) q :
+  {{{ ▷ l ↦{q} v }}}
+    type.load_ty_e #t #l
+  {{{ RET #v; l ↦{q} v }}}.
+Proof.
+  rewrite type.load_ty_e_unseal /=.
+  rewrite typed_pointsto_unseal /typed_pointsto_def.
+  pose proof (to_val_has_go_type v) as Hty.
+  generalize dependent (# v). clear dependent V.
+  induction t using go_type_ind;
+    iIntros (v Hty Φ) "Hl HΦ";
+    wp_call;
+    try solve [
+        inv Hty;
+        rewrite to_val_unseal /= ?loc_add_0 ?right_id;
+        iApply (wp_load with "[$Hl]");
+        iFrame
+      ].
+  - destruct (decide (uint.Z n = 0)).
+    + rewrite bool_decide_eq_true_2; [ wp_pures | word ].
+      assert (n = W64 0) by word; subst.
+      inv Hty; simpl.
+      assert (a = []) by (destruct a; naive_solver); subst; simpl.
+      rewrite to_val_unseal /=.
+      iApply "HΦ". iFrame.
+    + (* TODO: some sort of induction over uint.nat n needs to be started *)
+      rewrite bool_decide_eq_false_2; [ wp_pures | word ].
+      inv Hty.
+      destruct a as [|t' a']; simpl in *; [ word | ].
+      assert (has_go_type t' g) by naive_solver.
+      rewrite big_sepL_app.
+      iDestruct "Hl" as "[Hl1 Hl2]".
+      wp_apply (IHg with "[$Hl1]").
+      { auto. }
+      iIntros "Hl1".
+      wp_pures.
+      admit.
+  - inv Hty.
+    destruct i;
+      rewrite to_val_unseal /= ?loc_add_0 ?right_id;
+      iApply (wp_load with "[$Hl]");
+      iFrame.
+  - (* structT *)
+    admit.
+Admitted.
 
 End goose_lang.
